{
    "@context": {
        "rdf": "https://www.w3.org/1999/02/22-rdf-syntax-ns#",
        "rdfs": "http://www.w3.org/2000/01/rdf-schema#",
        "owl": "http://www.w3.org/2002/07/owl#",
        "dcterms": "http://purl.org/dc/terms/",
        "api": "http://zenomt.com/ns/terse-api#"
    },

    "@id": "http://zenomt.com/ns/terse-api",
    "@type": "owl:Ontology",
    "dcterms:title": "Vocabulary for the Terse JSON-LD API.",
    "rdfs:seeAlso": { "@id": "https://zenomt.github.io/jsonld-terse/api.html" },

    "@included": [
        {
            "@id": "api:Resource",
            "@type": "rdfs:Class",
            "rdfs:subClassOf": { "@id": "rdfs:Resource" },
            "rdfs:comment": "An HTTP-addressable resource conforming to the Terse JSON-LD API."
        },
        {
            "@id": "api:Page",
            "@type": "rdfs:Class",
            "rdfs:subClassOf": { "@id": "api:Resource" },
            "rdfs:comment": "A resource that is an in-sequence page of a paged resource as defined by the Terse JSON-LD API."
        },
        {
            "@id": "api:firstPage",
            "@type": "rdfs:Property",
            "rdfs:subPropertyOf": { "@id": "dcterms:hasPart" },
            "rdfs:domain": { "@id": "rdfs:Resource" },
            "rdfs:range": { "@id": "api:Page" },
            "rdfs:comment": "The first page of a paged resource."
        },
        {
            "@id": "api:lastPage",
            "@type": "rdfs:Property",
            "rdfs:subPropertyOf": { "@id": "dcterms:hasPart" },
            "rdfs:domain": { "@id": "rdfs:Resource" },
            "rdfs:range": { "@id": "api:Page" },
            "rdfs:comment": "The last page of a paged resource."
        },
        {
            "@id": "api:nextPage",
            "@type": "rdfs:Property",
            "rdfs:domain": { "@id": "api:Page" },
            "rdfs:range": { "@id": "api:Page" },
            "rdfs:comment": "The next in-sequence page of a paged resource."
        },
        {
            "@id": "api:prevPage",
            "@type": "rdfs:Property",
            "rdfs:domain": { "@id": "api:Page" },
            "rdfs:range": { "@id": "api:Page" },
            "rdfs:comment": "The previous in-sequence page of a paged resource."
        },
        {
            "@id": "api:pageOf",
            "@type": "rdfs:Property",
            "rdfs:subPropertyOf": { "@id": "dcterms:isPartOf" },
            "rdfs:domain": { "@id": "api:Page" },
            "rdfs:range": { "@id": "rdfs:Resource" },
            "rdfs:comment": "The resource of which the subject is a page."
        },
        {
            "@id": "api:View",
            "@type": "rdfs:Class",
            "rdfs:subClassOf": { "@id": "rdfs:Resource" },
            "rdfs:comment": "A resource (like the result of a QUERY) that is a view or projection of another resource."
        },
        {
            "@id": "api:viewOf",
            "@type": "rdfs:Property",
            "rdfs:subPropertyOf": { "@id": "dcterms:source" },
            "rdfs:domain": { "@id": "api:View" },
            "rdfs:range": { "@id": "rdfs:Resource" },
            "rdfs:comment": "The resource of which the subject is a view or projection."
        },
        {
            "@id": "api:etag",
            "@type": "rdfs:Property",
            "rdfs:domain": { "@id": "rdfs:Resource" },
            "rdfs:range": { "@id": "rdfs:Literal" },
            "rdfs:comment": "An entity-tag of the subject resource, including the double-quote characters."
        },
        {
            "@id": "api:Container",
            "@type": "rdfs:Class",
            "rdfs:subClassOf": [ { "@id": "api:Resource" }, { "@id": "rdfs:Container" }, { "@id": "rdf:Bag" } ],
            "rdfs:comment": "A Terse JSON-LD API unordered container."
        },
        {
            "@id": "api:member",
            "@type": "rdfs:Property",
            "rdfs:subPropertyOf": { "@id": "rdfs:member" },
            "rdfs:domain": { "@id": "api:Container" },
            "rdfs:range": { "@id": "api:Resource" },
            "rdfs:comment": "A member of a Container."
        },
        {
            "@id": "api:containerOf",
            "@type": "rdfs:Property",
            "rdfs:domain": { "@id": "api:Container" },
            "rdfs:range": { "@id": "rdfs:Class" },
            "rdfs:comment": "One of the expected types for members of the subject container."
        },
        {
            "@id": "api:Any",
            "@type": "rdfs:Class",
            "rdfs:subClassOf": { "@id": "rdfs:Resource" },
            "rdfs:comment": "The class of wildcards that match anything."
        },
        {
            "@id": "api:any",
            "@type": "api:Any",
            "rdfs:comment": "I am a wildcard that matches any URI, blank node, or literal."
        },
        {
            "@id": "api:Problem",
            "@type": "rdfs:class",
            "rdfs:subClassOf": { "@id": "rdfs:Resource" },
            "rdfs:comment": "A detailed description of an HTTP error response. My subclasses are more specific error types."
        },
        {
            "@id": "api:Action",
            "@type": "rdfs:class",
            "rdfs:subClassOf": { "@id": "api:Resource" },
            "rdfs:comment": "The class of actions (including event and webhook callbacks) that can be invoked by HTTP POST. An action is expected to have side effects on other resources. Concrete subclasses define the meaning of the action, and constraints or expectations on the POST request, if any. Membership in this class is implied by the rdfs:range of a concrete api:action sub-property. Membership in this class makes no implication on the semantics of the URI for methods other than POST."
        },
        {
            "@id": "api:IdempotentAction",
            "@type": "rdfs:class",
            "rdfs:subClassOf": { "@id": "api:Action" },
            "rdfs:comment": "The class of Actions that are idempotent."
        },
        {
            "@id": "api:action",
            "@type": "rdfs:Property",
            "owl:inverseOf": { "@id": "api:target" },
            "rdfs:domain": { "@id": "rdfs:Resource" },
            "rdfs:range": { "@id": "api:Action" },
            "rdfs:comment": "An HTTP POST to the object's URI invokes the action indicated by the concrete sub-property's rdfs:range on, or in the context of, the subject."
        },
        {
            "@id": "api:target",
            "@type": "rdfs:Property",
            "owl:inverseOf": { "@id": "api:action" },
            "rdfs:domain": { "@id": "api:Action" },
            "rdfs:range": { "@id": "rdfs:Resource" },
            "rdfs:comment": "The resource on which the Action acts."
        }
    ]
}
